Sha3/OfFnWorkaround.lean
@@ -1,0 +1,53 @@
+def Array.ofFn' {n} (f : Fin n → α) : Array α := go (Array.emptyWithCapacity n) n (Nat.le_refl n) where
+  go (acc : Array α) : (i : Nat) → i ≤ n → Array α
+  | i + 1, h =>
+     have w : n - i - 1 < n :=
+       Nat.lt_of_lt_of_le (Nat.sub_one_lt (Nat.sub_ne_zero_iff_lt.mpr h)) (Nat.sub_le n i)
+     go (acc.push (f ⟨n - i - 1, w⟩)) i (Nat.le_of_succ_le h)
+  | 0, _ => acc
+
+@[simp] theorem Array.size_ofFn'_go {n} {f : Fin n → α} {i acc h} :
+    (ofFn'.go f acc i h).size = acc.size + i := by
+  induction i generalizing acc with
+  | zero => simp [ofFn'.go]
+  | succ i ih =>
+    simpa [ofFn'.go, ih] using Nat.succ_add_eq_add_succ acc.size i
+@[simp] theorem Array.size_ofFn' {n : Nat} {f : Fin n → α} : (ofFn' f).size = n := by simp [ofFn']
+
+theorem Array.getElem_ofFn'_go {f : Fin n → α} {acc: Array α}{i k}(h : i ≤ n) (w₁ : k < acc.size + i) :
+    (ofFn'.go f acc i h)[k]'(by simpa using w₁) =
+      if w₂ : k < acc.size then acc[k] else f ⟨n - i + k - acc.size, by omega⟩ := by
+  induction i generalizing acc k with
+  | zero =>
+    simp at w₁
+    simp_all [ofFn'.go]
+  | succ i ih =>
+    unfold ofFn'.go
+    rw [ih]
+    · simp only [Array.size_push]
+      split <;> rename_i h'
+      · rw [Array.getElem_push]
+        split
+        · rfl
+        · congr 2
+          omega
+      · split
+        · omega
+        · congr 2
+          omega
+    · simp
+      omega
+
+@[simp] theorem Array.getElem_ofFn' {f : Fin n → α} {i : Nat} (h : i < (ofFn' f).size) :
+    (ofFn' f)[i] = f ⟨i, Array.size_ofFn' (f := f) ▸ h⟩ := by
+  unfold ofFn'
+  rw [getElem_ofFn'_go] <;> simp_all
+
+@[inline] def Vector.ofFn' (f : Fin n → α) : Vector α n := ⟨Array.ofFn' f, by simp⟩
+
+@[simp] theorem Vector.getElem_ofFn' {f : Fin n → α} {i : Nat} (h : i < n) :
+    (Vector.ofFn' f)[i] = f ⟨i, h⟩ := by
+  unfold ofFn'; rw [Vector.getElem_mk, Array.getElem_ofFn']
+
+@[simp] theorem Vector.getElem!_ofFn' [Inhabited α]{f : Fin n → α} {i : Nat} (h : i < n) :
+    (Vector.ofFn' f)[i]! = f ⟨i, h⟩ := by rw [getElem!_pos, Vector.getElem_ofFn']
